Spec.P256: tentative to output serialized points

specs/Spec.P256.fst
@@ -140,16 +140,15 @@ let scalar_multiplication k p =
   _norm q
 
 
-val secret_to_public: k: scalar -> Tot point_nat
-
-let secret_to_public k =
+val secret_to_public_raw: k: scalar -> Tot point_nat
+let secret_to_public_raw k =
   let pai = (0, 0, 0) in
   let basePoint = (0x6B17D1F2E12C4247F8BCE6E563A440F277037D812DEB33A0F4A13945D898C296, 0x4FE342E2FE1A7F9B8EE7EB4A7C0F9E162BCE33576B315ECECBB6406837BF51F5, 1) in
   let q, f = montgomery_ladder_spec k (pai, basePoint) in
   _norm q
 
-val isPointOnCurve: p: point_nat -> Tot bool
 
+val isPointOnCurve: p: point_nat -> Tot bool
 let isPointOnCurve p =
   let (x, y, z) = p in
   if (y * y) % prime = (x * x * x - 3 * x + 41058363725152142129326129780047268409114441015993725554835256314039467401291) % prime then
@@ -159,8 +158,8 @@ let isPointOnCurve p =
 
 type serialized_point = lbytes 64
 
-val serialize_point: point_nat -> serialized_point
-let serialize_point p =
+val point_to_serialized: point_nat -> serialized_point
+let point_to_serialized p =
   let np = _norm p in
   let (px0, py0, pz0) = np in
   assert_norm(prime256 < pow2 256);
@@ -171,3 +170,24 @@ let serialize_point p =
   let px8: lbytes 32 = Lib.ByteSequence.uints_to_bytes_le (Hacl.Spec.ECDSAP256.Definition.nat_as_seq px) in
   let py8: lbytes 32 = Lib.ByteSequence.uints_to_bytes_le (Hacl.Spec.ECDSAP256.Definition.nat_as_seq py) in
   (concat px8 py8)
+
+val serialized_to_point: serialized_point -> Tot point_nat
+let serialized_to_point p =
+  let px8 = sub p 0 32 in
+  let py8 = sub p 32 32 in
+  let px64 = Lib.ByteSequence.uints_from_bytes_le px8 in
+  let py64 = Lib.ByteSequence.uints_from_bytes_le py8 in
+  let px = Hacl.Spec.ECDSAP256.Definition.felem_seq_as_nat px64 in
+  let py = Hacl.Spec.ECDSAP256.Definition.felem_seq_as_nat py64 in
+  (px, py, 1)
+
+
+val scalarmult: k:scalar -> p:serialized_point -> Tot serialized_point
+let scalarmult k p =
+  let o = scalar_multiplication k (serialized_to_point p) in
+  point_to_serialized o
+
+val secret_to_public: k:scalar -> Tot serialized_point
+let secret_to_public k =
+  let o = secret_to_public_raw k in
+  point_to_serialized o
